iterative_HSem

FMap-HOLCF.thy
@@ -1094,31 +1094,35 @@ proof-
     by (metis fmap_below_dom)
 qed
 
-
-lemma iterative_fmap_add:
-  fixes \<rho> :: "('a::discrete_cpo, 'b::pcpo) fmap"
+locale iterative =
+  fixes \<rho> :: "('a::type, 'b::pcpo) fmap"
    and e1 :: "('a, 'b) fmap \<Rightarrow> ('a, 'b) fmap"
    and e2 :: "('a, 'b) fmap \<Rightarrow> 'b"
    and S :: "'a set" and x :: 'a
-  assumes [simp]:"cont e1"
-  assumes [simp]:"cont e2"
+   and D
+  defines "D \<equiv> insert x (fdom \<rho> \<union> S)"
+  assumes cont_e1 [simp]:"cont e1"
+  assumes cont_e2 [simp]:"cont e2"
   assumes dom[simp]: "\<And> \<rho>. fdom (e1 \<rho>) = S"
   assumes ne:"x \<notin> S"
-  defines "D \<equiv> (fdom \<rho> \<union> insert x S)"
-  shows "fix_on' (fmap_bottom D) (\<lambda> \<rho>'. (\<rho> f++ e1 \<rho>')(x f\<mapsto> e2 \<rho>')) =
-         fix_on' (fmap_bottom D) (\<lambda> \<rho>'. (\<rho> f++ fmap_restr S (fix_on' (fmap_bottom D) (\<lambda> \<rho>''. \<rho>' f++ e1 \<rho>'')))(x f\<mapsto> e2 \<rho>'))"
-        (is "fix_on' ?b ?L = fix_on' ?b ?R")
-proof(rule below_antisym)
-  let ?cpo = "{x. fmap_bottom D \<sqsubseteq> x}"
-  let ?H = "\<lambda> \<rho>' \<rho>''. \<rho>' f++ e1 \<rho>''"
 
-  have [simp]: "finite S" using dom[of undefined] by (auto simp del: dom)
-  have [simp]: "finite D" by (simp add: D_def)
+sublocale iterative < subpcpo "{x. fmap_bottom D \<sqsubseteq> x}" by (rule subpcpo_cone_above)
 
-  interpret subpcpo ?cpo by (rule subpcpo_cone_above)
+context iterative
+begin
 
-  
-  have cond1: "fix_on_cond ?cpo ?b ?L"
+  lemma [simp]: "finite S" using dom[of undefined] by (auto simp del: dom)
+  lemma [simp]: "finite D" by (simp add: D_def)
+ 
+
+  abbreviation "cpo == {x. fmap_bottom D \<sqsubseteq> x}"
+  abbreviation "b == fmap_bottom D"
+
+  abbreviation "L == (\<lambda> \<rho>'. (\<rho> f++ e1 \<rho>')(x f\<mapsto> e2 \<rho>'))"
+  abbreviation "H == (\<lambda> \<rho>' \<rho>''. \<rho>' f++ e1 \<rho>'')"
+  abbreviation "R == (\<lambda> \<rho>'. (\<rho> f++ fmap_restr S (fix_on' (fmap_bottom D) (H \<rho>')))(x f\<mapsto> e2 \<rho>'))"
+
+  lemma condL: "fix_on_cond cpo b L"
     apply (rule fix_on_condI)
     apply (rule subpcpo_cone_above)
     apply (rule bottom_of_cone_above)
@@ -1127,9 +1131,9 @@ proof(rule below_antisym)
     apply (rule cont_is_cont_on)
       apply simp
     done
-  note [simp] = fdom_fix_on[OF cond1]
+  lemmas [simp] = fdom_fix_on[OF condL]
 
-  have cond3: "\<And> \<rho>'. \<rho>' \<in> ?cpo \<Longrightarrow> fix_on_cond ?cpo ?b (?H \<rho>')"
+  lemma condH: "\<And> \<rho>'. \<rho>' \<in> cpo \<Longrightarrow> fix_on_cond cpo b (H \<rho>')"
     apply (rule fix_on_condI)
     apply (rule subpcpo_cone_above)
     apply (rule bottom_of_cone_above)
@@ -1138,18 +1142,18 @@ proof(rule below_antisym)
     apply (rule cont_is_cont_on)
       apply simp
     done
-  note [simp] = fdom_fix_on[OF cond3]
-
-  have cond2: "fix_on_cond ?cpo ?b ?R"
+  lemmas [simp] = fdom_fix_on[OF condH]
+  
+  lemma condR: "fix_on_cond cpo b R"
     apply (rule fix_on_condI)
     apply (rule subpcpo_cone_above)
     apply (rule bottom_of_cone_above)
     apply (rule closed_onI)
-      using fdom_fix_on[OF cond3]  apply (auto simp add: D_def)[1]
+      using fdom_fix_on[OF condH]  apply (auto simp add: D_def)[1]
     apply (rule cont_comp_cont_on2[OF cont2cont_lambda[OF fmap_upd_cont[OF cont_id cont_const]]
                 fmap_upd_cont[OF cont_const cont_id]
                 _
-                cont_is_cont_on[OF `cont e2`]])
+                cont_is_cont_on[OF cont_e2]])
     apply (rule cont_comp_cont_on2[OF cont2cont_lambda[OF fmap_add_cont1]
                 fmap_add_cont2
                 cont_is_cont_on[OF cont_const]
@@ -1157,127 +1161,133 @@ proof(rule below_antisym)
     apply (rule cont_comp_cont_on[OF fmap_restr_cont])
     apply (rule cont_onI2)
       apply (rule monofun_onI)
-      apply (erule (1) fix_on_mono[OF cond3 cond3])
+      apply (erule (1) fix_on_mono[OF condH condH])
       apply (erule cont2monofunE[OF fmap_add_cont1])
 
     apply (rule eq_imp_below)
-    apply (rule fix_on_cont[OF chain_on_is_chain cond3[OF chain_on_is_on]])
+    apply (rule fix_on_cont[OF chain_on_is_chain condH[OF chain_on_is_on]])
       apply assumption
       apply assumption
     apply (rule cont2cont_lambda[OF fmap_add_cont1])
     done
-  note [simp] = fdom_fix_on[OF cond2]
+  lemmas [simp] = fdom_fix_on[OF condR]
 
-  have [simp]: "D \<inter> S = S" 
-    by (auto simp add: D_def)
 
-  { fix y \<rho>
-    assume "y \<notin> S" and there: "(\<rho> :: ('a, 'b) fmap) \<in> ?cpo"
-    hence "lookup (fix_on' ?b (?H \<rho>)) y = lookup \<rho> y"
-    apply (subst fix_on_eq[OF cond3[OF there]])
-    by simp
-  } note H_ignores_not_S = this
-
-  { fix \<rho> \<rho>'
-    assume there: "(\<rho> :: ('a, 'b) fmap) \<in> ?cpo"
-    assume "\<And> x. x \<in> S \<Longrightarrow> the (lookup (e1 \<rho>') x) \<sqsubseteq> the (lookup \<rho> x)"
-    hence "?H \<rho> \<rho>' \<sqsubseteq> \<rho>"
-      apply -
-      apply (rule fmap_belowI')
-      using there apply (auto simp add: D_def)[1]
-      apply (case_tac "x \<in> fdom (e1 \<rho>')")
-      apply simp
-      apply simp
-      done
-  } note H_noop = this
+  lemma iterative_fmap_add:
+    shows "fix_on' (fmap_bottom D) (\<lambda> \<rho>'. (\<rho> f++ e1 \<rho>')(x f\<mapsto> e2 \<rho>')) =
+           fix_on' (fmap_bottom D) (\<lambda> \<rho>'. (\<rho> f++ fmap_restr S (fix_on' (fmap_bottom D) (\<lambda> \<rho>''. \<rho>' f++ e1 \<rho>'')))(x f\<mapsto> e2 \<rho>'))"
+  proof(rule below_antisym)
+    have [simp]: "D \<inter> S = S" 
+      by (auto simp add: D_def)
   
-  note fix_eq_R = fix_on_eq[OF cond2]
-  note fix_eq_L = fix_on_eq[OF cond1]
-  note fix_eq_HR = fix_on_eq[OF cond3[OF fix_on_there[OF cond2]]]
-
-  have HR_not_S[simp]: "\<And> x. x \<notin> S \<Longrightarrow> lookup (fix_on' ?b (?H (fix_on' ?b ?R))) x = lookup (fix_on' ?b ?R) x"
-    apply (subst fix_eq_HR) by simp
-
-  have HR_S[simp]: "\<And> y. y \<in> S \<Longrightarrow> lookup (fix_on' ?b (?H (fix_on' ?b ?R))) y = lookup (e1 (fix_on' ?b (?H (fix_on' ?b ?R)))) y"
-    apply (subgoal_tac "y \<noteq> x")
-    apply (subst fix_eq_HR)
-    apply simp
-    using ne by metis
-
-  have L_S[simp]: "\<And> y. y \<in> S \<Longrightarrow> lookup (fix_on' ?b ?L) y = lookup (e1 (fix_on' ?b ?L)) y"
-    apply (subgoal_tac "y \<noteq> x")
-    apply (subst (1) fix_eq_L)
-    apply simp
-    using ne by metis
-
-  have L_x2[simp]: "the (lookup (fix_on' ?b ?L) x) = e2 (fix_on' ?b ?L)"
-    by (subst (1) fix_eq_L, simp)
-
-  have L_not_S_x2[simp]: "\<And> y. y \<notin> S \<Longrightarrow> y \<noteq> x \<Longrightarrow> lookup (fix_on' ?b ?L) y = lookup \<rho> y"
-    by (subst (1) fix_eq_L, simp)
-
-  have R_S[simp]: "\<And> y. y \<in> S \<Longrightarrow> lookup (fix_on' ?b ?R) y = lookup (e1 (fix_on' ?b (?H (fix_on' ?b ?R)))) y"
-    apply (subgoal_tac "y \<noteq> x")
-    apply (subst fix_eq_R)
-    apply simp
-    using ne by metis
-
-  have R_x2[simp]: "the (lookup (fix_on' ?b ?R) x) = e2 (fix_on'?b ?R)"
-    by (subst fix_eq_R, simp)
-
-  have R_not_S[simp]: "\<And> y. y \<notin> S \<Longrightarrow> y \<noteq> x \<Longrightarrow> lookup (fix_on' ?b ?R) y = lookup \<rho> y"
-    by (subst fix_eq_R, simp)
-
-  have HR_is_R[simp]: "fix_on' ?b (?H (fix_on' ?b ?R)) = fix_on' ?b ?R"
-    apply (rule fmap_eqI)
-    apply simp
-    apply (case_tac "xa \<in> S")
-    apply simp_all
-    done
-
-  have HLL_below_L: "?H (fix_on' ?b ?L) (fix_on' ?b ?L) \<sqsubseteq> (fix_on' ?b ?L)"
-    by (rule H_noop, simp_all)
-
-  show "fix_on' ?b ?R \<sqsubseteq> fix_on' ?b ?L"
-  proof (rule fix_on_least_below[OF cond2])
-    show "fix_on' ?b ?L \<in> ?cpo"
+    { fix y \<rho>
+      assume "y \<notin> S" and there: "(\<rho> :: ('a, 'b) fmap) \<in> cpo"
+      hence "lookup (fix_on' b (H \<rho>)) y = lookup \<rho> y"
+      apply (subst fix_on_eq[OF condH[OF there]])
       by simp
-    show "?R (fix_on' ?b ?L) \<sqsubseteq> fix_on' ?b ?L"
-    proof(rule fmap_upd_belowI)
-      case goal1 show ?case by (simp, auto simp add: D_def)
-      show "e2 (fix_on' ?b ?L) \<sqsubseteq> the (lookup (fix_on' ?b ?L) x)"
+    } note H_ignores_not_S = this
+  
+    { fix \<rho> \<rho>'
+      assume there: "(\<rho> :: ('a, 'b) fmap) \<in> cpo"
+      assume "\<And> x. x \<in> S \<Longrightarrow> the (lookup (e1 \<rho>') x) \<sqsubseteq> the (lookup \<rho> x)"
+      hence "H \<rho> \<rho>' \<sqsubseteq> \<rho>"
+        apply -
+        apply (rule fmap_belowI')
+        using there apply (auto simp add: D_def)[1]
+        apply (case_tac "x \<in> fdom (e1 \<rho>')")
+        apply simp
+        apply simp
+        done
+    } note H_noop = this
+    
+    note fix_eq_R = fix_on_eq[OF condR]
+    note fix_eq_L = fix_on_eq[OF condL]
+    note fix_eq_HR = fix_on_eq[OF condH[OF fix_on_there[OF condR]]]
+  
+    have HR_not_S[simp]: "\<And> x. x \<notin> S \<Longrightarrow> lookup (fix_on' b (H (fix_on' b R))) x = lookup (fix_on' b R) x"
+      apply (subst fix_eq_HR) by simp
+  
+    have HR_S[simp]: "\<And> y. y \<in> S \<Longrightarrow> lookup (fix_on' b (H (fix_on' b R))) y = lookup (e1 (fix_on' b (H (fix_on' b R)))) y"
+      apply (subgoal_tac "y \<noteq> x")
+      apply (subst fix_eq_HR)
+      apply simp
+      using ne by metis
+  
+    have L_S[simp]: "\<And> y. y \<in> S \<Longrightarrow> lookup (fix_on' b L) y = lookup (e1 (fix_on' b L)) y"
+      apply (subgoal_tac "y \<noteq> x")
+      apply (subst (1) fix_eq_L)
+      apply simp
+      using ne by metis
+  
+    have L_x2[simp]: "the (lookup (fix_on' b L) x) = e2 (fix_on' b L)"
+      by (subst (1) fix_eq_L, simp)
+  
+    have L_not_S_x2[simp]: "\<And> y. y \<notin> S \<Longrightarrow> y \<noteq> x \<Longrightarrow> lookup (fix_on' b L) y = lookup \<rho> y"
+      by (subst (1) fix_eq_L, simp)
+  
+    have R_S[simp]: "\<And> y. y \<in> S \<Longrightarrow> lookup (fix_on' b R) y = lookup (e1 (fix_on' b (H (fix_on' b R)))) y"
+      apply (subgoal_tac "y \<noteq> x")
+      apply (subst fix_eq_R)
+      apply simp
+      using ne by metis
+  
+    have R_x2[simp]: "the (lookup (fix_on' b R) x) = e2 (fix_on' b R)"
+      by (subst fix_eq_R, simp)
+  
+    have R_not_S[simp]: "\<And> y. y \<notin> S \<Longrightarrow> y \<noteq> x \<Longrightarrow> lookup (fix_on' b R) y = lookup \<rho> y"
+      by (subst fix_eq_R, simp)
+  
+    have HR_is_R[simp]: "fix_on' b (H (fix_on' b R)) = fix_on' b R"
+      apply (rule fmap_eqI)
+      apply simp
+      apply (case_tac "xa \<in> S")
+      apply simp_all
+      done
+  
+    have HLL_below_L: "H (fix_on' b L) (fix_on' b L) \<sqsubseteq> (fix_on' b L)"
+      by (rule H_noop, simp_all)
+  
+    show "fix_on' b R \<sqsubseteq> fix_on' b L"
+    proof (rule fix_on_least_below[OF condR])
+      show "fix_on' b L \<in> cpo"
         by simp
-      case (goal2 y)
-        hence [simp]:"y \<noteq> x" by metis
-      show "the (lookup (\<rho> f++ fmap_restr S (fix_on' ?b (?H (fix_on' ?b ?L)))) y) \<sqsubseteq> the (lookup (fix_on' ?b ?L) y)"
-      proof(cases "y \<in> S")
-      case True[simp]
-        from HLL_below_L
-        have "(fix_on' ?b (?H (fix_on' ?b ?L))) \<sqsubseteq> (fix_on' ?b ?L)"
-          by (rule fix_on_least_below[OF cond3[OF fix_on_there[OF cond1]] fix_on_there[OF cond1]])
-        hence "the (lookup (fix_on' ?b (?H (fix_on' ?b ?L))) y) \<sqsubseteq> the (lookup (fix_on' ?b ?L) y)"
-          by (rule fmap_belowE)
-        thus ?thesis
-          by (subst lookup_fmap_add1, simp_all)
-      next
-      case False
-        thus ?thesis by simp
+      show "R (fix_on' b L) \<sqsubseteq> fix_on' b L"
+      proof(rule fmap_upd_belowI)
+        case goal1 show ?case by (simp, auto simp add: D_def)
+        show "e2 (fix_on' b L) \<sqsubseteq> the (lookup (fix_on' b L) x)"
+          by simp
+        case (goal2 y)
+          hence [simp]:"y \<noteq> x" by metis
+        show "the (lookup (\<rho> f++ fmap_restr S (fix_on' b (H (fix_on' b L)))) y) \<sqsubseteq> the (lookup (fix_on' b L) y)"
+        proof(cases "y \<in> S")
+        case True[simp]
+          from HLL_below_L
+          have "(fix_on' b (H (fix_on' b L))) \<sqsubseteq> (fix_on' b L)"
+            by (rule fix_on_least_below[OF condH[OF fix_on_there[OF condL]] fix_on_there[OF condL]])
+          hence "the (lookup (fix_on' b (H (fix_on' b L))) y) \<sqsubseteq> the (lookup (fix_on' b L) y)"
+            by (rule fmap_belowE)
+          thus ?thesis
+            by (subst lookup_fmap_add1, simp_all)
+        next
+        case False
+          thus ?thesis by simp
+        qed
       qed
     qed
+  
+    show "fix_on' b L \<sqsubseteq> fix_on' b R"
+    proof (rule fix_on_least_below[OF condL])
+      show "fix_on' b R \<in> cpo"
+        by simp
+      show "L (fix_on' b R) \<sqsubseteq> fix_on' b R"
+        apply (rule  fmap_upd_belowI)
+        apply simp apply (auto simp add: D_def)[1]
+        apply (case_tac "z \<notin> S")
+        apply simp_all
+      done
+    qed
   qed
-
-  show "fix_on' ?b ?L \<sqsubseteq> fix_on' ?b ?R"
-  proof (rule fix_on_least_below[OF cond1])
-    show "fix_on' ?b ?R \<in> ?cpo"
-      by simp
-    show "?L (fix_on' ?b ?R) \<sqsubseteq> fix_on' ?b ?R"
-      apply (rule  fmap_upd_belowI)
-      apply simp apply (auto simp add: D_def)[1]
-      apply (case_tac "z \<notin> S")
-      apply simp_all
-    done
-  qed
-qed
+end
 
 instance fmap :: (type, Nonempty_Meet_cpo) Bounded_Nonempty_Meet_cpo
 apply default
